\begin{questions}
\question{ $$
u\text {满足 }\left\{\begin{array}{l}
u_{t t}-a^{2}\left(u_{x x}+u_{y y}\right)=0,\quad (x,y)\in \Omega ,t>0 \\
u(x, y, t)=0 ,\quad(x, y) \in \partial \Omega \\
u(x, y, 0)=\varphi(x, y) \\
u_{t}(x, y, 0)=\psi(x, y)
\end{array}\right.
$$
}
证明: 
$$
\begin{aligned}
&\iint_{\Omega}\left[u_{t} u_{t t}-a^{2}\left(u_{x x}+u_{y y}\right) u_{t}\right] d x d y\\
&=\frac{1}{2} \frac{d}{d t} \iint\limits_{\Omega} u_{t}^{2} d x d y-a^{2} \oint\limits_{\partial \Omega}\left(u_{x} u_{t} \cos (\vec{\boldsymbol n}, x)+u_{y} u_{t} \cos (\vec{\boldsymbol n}, y)\right) d s +a^{2} \iint\limits_{\Omega}\left(u_{x} u_{t x}+u_{y} u_{t y}\right) d x d y \\
&=\frac{1}{2} \frac{d}{d t} \iint\limits_{\Omega} u_{t}^{2} d x d y+\frac{a^{2}}{2} \frac{d}{d t} \iint\limits_{\Omega}\left(u_{x}^{2}+u_{y}^{2}\right) d x d y
\end{aligned}
$$
\begin{solution}
$$
\text { 由 } \frac{d}{d t}\left(u_{t}^{2}\right)=2 u_{t} \cdot u_{t t} \text { 知 } \iint_{\Omega} u_{t} u_{t t} d x d y=\frac{1}{2} \frac{d}{d t} \iint\limits_{\Omega} u_{t}^{2}
$$
$$\text { 且有 } \Delta u=u_{x x}+u_{y y}$$

利用方向导数的计算公式
$$\frac{\partial u}{\partial \vec{\boldsymbol n}}=\frac{\partial u}{\partial x} \cdot \cos (\vec{\boldsymbol n}, x)+\frac{\partial u}{\partial y} \cdot \cos (\vec{\boldsymbol n}, y) $$
我们计算如下：
$$
\begin{aligned}
a^{2} \oint\limits_{\partial \Omega}u_{t} \cdot \frac{\partial u}{\partial \vec{\boldsymbol n}} d s&=a^{2} \oint\limits_{\partial \Omega} u_{t}\left[\frac{\partial u}{\partial x} \cdot \cos (\vec{\boldsymbol n}, x)+\frac{\partial u}{\partial y} \cdot \cos (\vec{\boldsymbol n} \cdot y)\right] d s \\
&= a^{2} \oint\limits_{\partial \Omega} u_{t} \frac{\partial u}{\partial x} d y-u_{t} \frac{\partial u}{\partial y} d x \\
\end{aligned}
$$
令$P=-u_{t} \cdot \frac{\partial u}{\partial y} ,\quad Q=u_{t} \cdot \frac{\partial u}{\partial x}$,
则由格林公式得
$$
\begin{aligned}
a^{2} \oint\limits_{\partial \Omega}u_{t} \cdot \frac{\partial u}{\partial \vec{\boldsymbol n}} d S&=a^{2} \iint\limits_{\Omega} \left[\frac{\partial}{\partial x}\left(u_{t} \frac{\partial u}{\partial x}\right)+\frac{\partial}{\partial y}\left(u_{t} \frac{\partial u}{\partial y}\right)\right] d x d y \\
&=a^{2} \iint\limits_{\Omega}\left(u_{t x} \cdot \frac{\partial u}{\partial x}+u_{t} \frac{\partial^{2} u}{\partial x^{2}}+u_{t y} \frac{\partial u}{\partial y}+u_{t} \cdot \frac{\partial^{2} u}{\partial y^{2}}\right) d x d y \\
&=a^{2} \iint\limits_{\Omega}\left(u_{t x} u_{x}+u_{t y} u_{y}+u_{t} \Delta u\right) d x d y \\
&=a^{2} \iint\limits_{\Omega}\left(u_{x} u_{t x}+u_{y} u_{t y}\right) d x d y+a^{2} \iint\limits _{\Omega} u_{t} \Delta u d x d y
\end{aligned}
$$
因此 
$$ a^{2} \iint\limits_{\Omega} u_{t} \Delta u d x d y=a^{2} \oint\limits_{\partial \Omega} u_{t} \frac{\partial u}{\partial \vec{\boldsymbol n}} d s-a^{2} \iint\limits_{\Omega}\left(u_{x} u_{tx} +u_{y} u_{t y}\right) d x d y $$ 
由于 $ u(x, y, t)=0 ,\quad(x, y) \in \partial \Omega $
则 $ \left.u_{t}\right|_{\partial \Omega}=0 $.
即有 $$ a^{2} \iint\limits_{\Omega} u_{t} \Delta u d x d y=-a^{2} \iint\limits_{\Omega}\left(u_{x} u_{t x}+u_{y} u_{t y}\right) d x d y $$
 注意到 $ \frac{d}{d t}\left(u_{x}^{2}+u_{y}^{2}\right)=2\left(u_{x} u_{t x}+u_{y} u_{t y}\right) $
$$
\Rightarrow a^{2} \iint\limits_{\Omega}\left(u_{x} u_{t x}+u_{y} u_{t y}\right) d x d y=\frac{a^{2}}{2} \frac{d}{d t} \iint\limits_{\Omega}\left(u_{x}^{2}+u_{y}^{2}\right) d x d y
$$
因此得证.

\end{solution}
\end{questions}